avoid extra copy for fsum and fdifference

code/ed25519/Hacl.Impl.Ed25519.RecoverX.fst
@@ -20,48 +20,10 @@ module SE = Spec.Ed25519
 inline_for_extraction noextract
 let elemB = lbuffer uint64 5ul
 
-inline_for_extraction noextract
-val recover_x_step_1:
-    x2:elemB
-  -> y:elemB ->
-  Stack unit
-    (requires fun h -> live h x2 /\ live h y /\ disjoint x2 y /\
-      F51.mul_inv_t h y
-    )
-    (ensures  fun h0 _ h1 -> modifies (loc x2) h0 h1 /\
-      F51.fevalh h1 x2 == F51.as_nat h1 x2 /\
-      F51.mul_inv_t h1 x2 /\
-      (let y = F51.fevalh h0 y in
-       let x2 = F51.fevalh h1 x2 in
-       let y2 = y `SC.fmul` y in
-       x2 == (y2 `SC.fsub` SC.one) `SC.fmul` (SC.finv ((SE.d `SC.fmul` y2) `SC.fadd` SC.one)))
-    )
-let recover_x_step_1 x2 y =
-  push_frame();
-  let tmp = create 25ul (u64 0) in
-  let one = sub tmp 0ul 5ul in
-  let y2  = sub tmp 5ul 5ul in
-  let dyyi = sub tmp 10ul 5ul in
-  let dyy = sub tmp 15ul 5ul in
-  make_one one;
-  fsquare y2 y; // y2 = y `fmul` y
-  times_d dyy y2; // dyy = d `fmul` (y `fmul` y)
-  fsum dyy one;   // dyy = (d `fmul` (y `fmul` y)) `fadd` one
-  reduce_513 dyy;
-  inverse dyyi dyy; // dyyi = modp_inv ((d `fmul` (y `fmul` y)) `fadd` one)
-  fdifference one y2; // one = (y `fmul` y) `fsub` 1
-  fmul x2 one dyyi; //
-  reduce x2;
-  pop_frame()
-
-
-val is_0:
-  x:elemB ->
-  Stack bool
-    (requires fun h -> live h x /\ F51.as_nat h x == F51.fevalh h x)
-    (ensures  fun h0 b h1 -> h0 == h1 /\
-      (b <==> (F51.fevalh h0 x == SC.zero))
-    )
+val is_0: x:elemB -> Stack bool
+  (requires fun h -> live h x /\ F51.as_nat h x == F51.fevalh h x)
+  (ensures  fun h0 b h1 -> h0 == h1 /\
+    (b <==> (F51.fevalh h0 x == SC.zero)))
 
 [@CInline]
 let is_0 x =
@@ -79,37 +41,13 @@ let is_0 x =
    u64_to_UInt64 x4 =^ 0uL)
 
 
-val mul_modp_sqrt_m1:
-  x:elemB ->
-  Stack unit
-    (requires fun h -> live h x /\ F51.mul_inv_t h x)
-    (ensures  fun h0 _ h1 -> modifies (loc x) h0 h1 /\
-      F51.mul_inv_t h1 x /\
-      F51.fevalh h1 x == F51.fevalh h0 x `SC.fmul` SE.modp_sqrt_m1
-    )
-
-[@CInline]
-let mul_modp_sqrt_m1 x =
-  push_frame();
-  let sqrt_m1 = create 5ul (u64 0) in
-  make_u64_5 sqrt_m1
-    (u64 0x00061b274a0ea0b0) (u64 0x0000d5a5fc8f189d) (u64 0x0007ef5e9cbd0c60) (u64 0x00078595a6804c9e) (u64 0x0002b8324804fc1d);
-
-  assert_norm (S51.as_nat5 (u64 0x00061b274a0ea0b0, u64 0x0000d5a5fc8f189d, u64 0x0007ef5e9cbd0c60, u64 0x00078595a6804c9e, u64 0x0002b8324804fc1d) == SE.modp_sqrt_m1);
-  fmul x x sqrt_m1;
-  pop_frame()
-
-
 inline_for_extraction noextract
-val gte_q:
-  x:elemB ->
-  Stack bool
-    (requires fun h -> live h x /\
-      F51.felem_fits h x (1, 1, 1, 1, 1)
-    )
-    (ensures  fun h0 b h1 -> h0 == h1 /\
-      (b <==> (F51.as_nat h0 x >= SC.prime))
-    )
+val gte_q: x:elemB -> Stack bool
+  (requires fun h -> live h x /\
+    F51.felem_fits h x (1, 1, 1, 1, 1))
+  (ensures  fun h0 b h1 -> h0 == h1 /\
+    (b <==> (F51.as_nat h0 x >= SC.prime)))
+
 let gte_q x =
   let open Lib.RawIntTypes in
   let open FStar.UInt64 in
@@ -125,16 +63,36 @@ let gte_q x =
    u64_to_UInt64 x4 =^ 0x7ffffffffffffuL)
 
 
+val mul_modp_sqrt_m1: x:elemB -> Stack unit
+  (requires fun h -> live h x /\ F51.mul_inv_t h x)
+  (ensures  fun h0 _ h1 -> modifies (loc x) h0 h1 /\
+    F51.mul_inv_t h1 x /\
+    F51.fevalh h1 x == F51.fevalh h0 x `SC.fmul` SE.modp_sqrt_m1)
+
+[@CInline]
+let mul_modp_sqrt_m1 x =
+  [@inline_let] let (x0, x1, x2, x3, x4) =
+    (u64 0x00061b274a0ea0b0,
+    u64 0x0000d5a5fc8f189d,
+    u64 0x0007ef5e9cbd0c60,
+    u64 0x00078595a6804c9e,
+    u64 0x0002b8324804fc1d) in
+
+  push_frame();
+  let sqrt_m1 = create 5ul (u64 0) in
+  make_u64_5 sqrt_m1 x0 x1 x2 x3 x4;
+  assert_norm (S51.as_nat5 (x0, x1, x2, x3, x4) == SE.modp_sqrt_m1);
+  fmul x x sqrt_m1;
+  pop_frame()
+
+
 inline_for_extraction noextract
-val x_mod_2:
-  x:felem ->
-  Stack uint64
-    (requires fun h -> live h x)
-    (ensures  fun h0 z h1 -> h0 == h1 /\ v z < 2 /\
-      v z == F51.as_nat h0 x % 2
-    )
+val x_mod_2: x:felem -> Stack uint64
+  (requires fun h -> live h x)
+  (ensures  fun h0 z h1 -> h0 == h1 /\ v z < 2 /\
+    v z == F51.as_nat h0 x % 2)
+
 let x_mod_2 x =
-  (**) let h0 = ST.get() in
   let x0 = x.(0ul) in
   let z  = x0 &. u64 1 in
   mod_mask_lemma x0 1ul;
@@ -143,154 +101,162 @@ let x_mod_2 x =
 
 
 inline_for_extraction noextract
-val recover_x_step_2:
-    x:elemB
-  -> sign:uint64
-  -> x2:elemB ->
-  Stack uint8
-    (requires fun h -> live h x2 /\ live h x /\ disjoint x x2 /\
-      F51.mul_inv_t h x /\
-      F51.fevalh h x2 == F51.as_nat h x2
-    )
-    (ensures  fun h0 z h1 -> modifies (loc x) h0 h1 /\
-      F51.mul_inv_t h1 x /\
-      (if F51.fevalh h0 x2 = 0 then (
-        if v sign = 0 then F51.fevalh h1 x = 0 /\ z == u8 1
-        else h0 == h1 /\ z == u8 0
-        )
-       else h0 == h1 /\ z == u8 2)
-    )
+val recover_x_step_1: x2:elemB -> y:elemB -> Stack unit
+  (requires fun h ->
+    live h x2 /\ live h y /\ disjoint x2 y /\
+    F51.mul_inv_t h y)
+  (ensures  fun h0 _ h1 -> modifies (loc x2) h0 h1 /\
+    F51.fevalh h1 x2 == F51.as_nat h1 x2 /\
+    F51.mul_inv_t h1 x2 /\
+    (let y = F51.fevalh h0 y in
+    let x2 = F51.fevalh h1 x2 in
+    let y2 = y `SC.fmul` y in
+    x2 == (y2 `SC.fsub` SC.one) `SC.fmul` (SC.finv ((SE.d `SC.fmul` y2) `SC.fadd` SC.one))))
+
+let recover_x_step_1 x2 y =
+  push_frame();
+  let tmp = create 20ul (u64 0) in
+  let one = sub tmp 0ul 5ul in
+  let y2  = sub tmp 5ul 5ul in
+  let dyyi = sub tmp 10ul 5ul in
+  let dyy = sub tmp 15ul 5ul in
+
+  make_one one;
+  fsquare y2 y;     // y2 = y * y
+  times_d dyy y2;   // dyy = d * y2
+  fsum dyy dyy one; // dyy = (d * y2) + one
+  reduce_513 dyy;
+  inverse dyyi dyy; // dyyi = modp_inv ((d * y2) + one)
+
+  fdifference x2 y2 one; // x2 = y2 - one
+  fmul x2 x2 dyyi;       // x2 = (y2 - one) * dyyi
+  reduce x2;
+  pop_frame()
+
+
+inline_for_extraction noextract
+val recover_x_step_2: x:elemB -> sign:uint64 -> x2:elemB -> Stack uint8
+  (requires fun h ->
+    live h x2 /\ live h x /\ disjoint x x2 /\
+    F51.mul_inv_t h x /\ F51.fevalh h x2 == F51.as_nat h x2)
+  (ensures  fun h0 z h1 -> modifies (loc x) h0 h1 /\
+    F51.mul_inv_t h1 x /\
+    (if F51.fevalh h0 x2 = 0 then (
+      if v sign = 0 then F51.fevalh h1 x = 0 /\ z == u8 1
+      else h0 == h1 /\ z == u8 0)
+     else h0 == h1 /\ z == u8 2))
+
 let recover_x_step_2 x sign x2 =
   let open Lib.RawIntTypes in
   let open FStar.UInt64 in
-  let h0 = ST.get() in
   let x2_is_0 = is_0 x2 in
-  let h1 = ST.get() in
-  if x2_is_0 then (
-    assert (uint_v #U64 sign = Lib.IntTypes.v #U64 #SEC sign);
-    if u64_to_UInt64 sign =^ 0uL then (
-      make_zero x;
-      u8 1
-    ) else u8 0
-  ) else u8 2
+  if x2_is_0 then begin
+    if u64_to_UInt64 sign =^ 0uL then (make_zero x; u8 1) else u8 0 end
+  else u8 2
+
 
 inline_for_extraction noextract
-val recover_x_step_3:
-  tmp:lbuffer uint64 20ul ->
-  Stack unit
-    (requires fun h -> live h tmp /\ F51.mul_inv_t h (gsub tmp 0ul 5ul))
-    (ensures  fun h0 _ h1 -> modifies (loc tmp) h0 h1 /\
-      F51.mul_inv_t h1 (gsub tmp 5ul 5ul) /\
-      F51.fevalh h0 (gsub tmp 0ul 5ul) == F51.fevalh h1 (gsub tmp 0ul 5ul) /\
-      F51.mul_inv_t h1 (gsub tmp 0ul 5ul) /\
-      (let x2 = F51.fevalh h0 (gsub tmp 0ul 5ul) in
-       let x = x2 `SC.fpow` ((SC.prime + 3) / 8) in
-       let x = if ((x `SC.fmul` x) `SC.fsub` x2) <> 0 then (x `SC.fmul` SE.modp_sqrt_m1) else x in
-       F51.fevalh h1 (gsub tmp 5ul 5ul) == x
-      )
-    )
+val recover_x_step_3: tmp:lbuffer uint64 15ul -> Stack unit
+  (requires fun h -> live h tmp /\ F51.mul_inv_t h (gsub tmp 0ul 5ul))
+  (ensures  fun h0 _ h1 -> modifies (loc tmp) h0 h1 /\
+    F51.mul_inv_t h1 (gsub tmp 5ul 5ul) /\
+    F51.fevalh h0 (gsub tmp 0ul 5ul) == F51.fevalh h1 (gsub tmp 0ul 5ul) /\
+    F51.mul_inv_t h1 (gsub tmp 0ul 5ul) /\
+    (let x2 = F51.fevalh h0 (gsub tmp 0ul 5ul) in
+    let x = x2 `SC.fpow` ((SC.prime + 3) / 8) in
+    let x = if ((x `SC.fmul` x) `SC.fsub` x2) <> 0 then (x `SC.fmul` SE.modp_sqrt_m1) else x in
+    F51.fevalh h1 (gsub tmp 5ul 5ul) == x))
+
 let recover_x_step_3 tmp =
   let x2  = sub tmp 0ul 5ul in
-  let x3  = sub tmp 5ul 5ul in
+  let x3  = sub tmp 5ul 5ul in // x
   let t0  = sub tmp 10ul 5ul in
-  let t1  = sub tmp 15ul 5ul in
-  Hacl.Impl.Ed25519.Pow2_252m2.pow2_252m2 x3 x2;
-  fsquare t0 x3;
-  copy t1 x2;
-  fdifference t1 t0;
-  reduce_513 t1;
-  reduce t1;
-  let t1_is_0 = is_0 t1 in
-  if t1_is_0 then ()
-  else (
-    mul_modp_sqrt_m1 x3
-  )
-//  reduce x3
+  Hacl.Impl.Ed25519.Pow2_252m2.pow2_252m2 x3 x2; // x3 = x2^((prime + 3) / 8)
+  fsquare t0 x3;        // t0 = x3 * x3
+  fdifference t0 t0 x2; // t0 = t0 - x2
+  reduce_513 t0;
+  reduce t0;
+  let t0_is_0 = is_0 t0 in
+  if t0_is_0 then () else mul_modp_sqrt_m1 x3
+
 
 inline_for_extraction noextract
-val recover_x_step_4:
-  tmp:lbuffer uint64 20ul ->
-  Stack bool
-    (requires fun h -> live h tmp /\
-      F51.mul_inv_t h (gsub tmp 0ul 5ul) /\
-      F51.mul_inv_t h (gsub tmp 5ul 5ul)
-    )
-    (ensures  fun h0 z h1 -> modifies (loc tmp) h0 h1 /\
-      F51.fevalh h0 (gsub tmp 0ul 5ul) == F51.fevalh h1 (gsub tmp 0ul 5ul) /\
-      F51.mul_inv_t h1 (gsub tmp 0ul 5ul) /\
-      F51.fevalh h0 (gsub tmp 5ul 5ul) == F51.fevalh h1 (gsub tmp 5ul 5ul) /\
-      F51.mul_inv_t h1 (gsub tmp 5ul 5ul) /\
-      (let u = F51.fevalh h0 (gsub tmp 5ul 5ul) in
-       let v = F51.fevalh h0 (gsub tmp 0ul 5ul) in
-       let y = (u `SC.fmul` u) `SC.fsub` v in
-       (z <==> y == SC.zero)
-      )
-    )
+val recover_x_step_4: tmp:lbuffer uint64 15ul -> Stack bool
+  (requires fun h -> live h tmp /\
+    F51.mul_inv_t h (gsub tmp 0ul 5ul) /\
+    F51.mul_inv_t h (gsub tmp 5ul 5ul))
+  (ensures  fun h0 z h1 -> modifies (loc tmp) h0 h1 /\
+    F51.fevalh h0 (gsub tmp 0ul 5ul) == F51.fevalh h1 (gsub tmp 0ul 5ul) /\
+    F51.mul_inv_t h1 (gsub tmp 0ul 5ul) /\
+    F51.fevalh h0 (gsub tmp 5ul 5ul) == F51.fevalh h1 (gsub tmp 5ul 5ul) /\
+    F51.mul_inv_t h1 (gsub tmp 5ul 5ul) /\
+    (let u = F51.fevalh h0 (gsub tmp 5ul 5ul) in
+    let v = F51.fevalh h0 (gsub tmp 0ul 5ul) in
+    let y = (u `SC.fmul` u) `SC.fsub` v in
+    (z <==> y == SC.zero)))
+
 let recover_x_step_4 tmp =
-  let h0 = ST.get() in
   let x2  = sub tmp 0ul 5ul in
   let x3  = sub tmp 5ul 5ul in
   let t0  = sub tmp 10ul 5ul in
-  let t1  = sub tmp 15ul 5ul in
-  fsquare t0 x3;
-  copy t1 x2;
-  fdifference t1 t0;
-  reduce_513 t1;
-  reduce t1;
-  is_0 t1
+  fsquare t0 x3;        // t0 = x3 * x3
+  fdifference t0 t0 x2; // t0 - x2
+  reduce_513 t0;
+  reduce t0;
+  is_0 t0
+
 
 inline_for_extraction noextract
 val recover_x_step_5:
     x:elemB
   -> y:elemB
   -> sign:uint64{v sign = 0 \/ v sign = 1}
-  -> tmp:lbuffer uint64 20ul ->
+  -> tmp:lbuffer uint64 15ul ->
   Stack unit
-    (requires fun h -> live h x /\ live h tmp /\ live h y /\
-      disjoint x y /\ disjoint tmp x /\ disjoint tmp y /\
-      F51.mul_inv_t h (gsub tmp 5ul 5ul) /\
-      (let y = F51.as_nat h y in
-       let sign = (uint_v #U64 sign <> 0) in
-       let x = F51.fevalh h (gsub tmp 5ul 5ul) in
-       let x2 = F51.fevalh h (gsub tmp  0ul 5ul) in
-       ((x `SC.fmul` x) `SC.fsub` x2) == SC.zero /\
-       SE.recover_x y sign ==
-           (if ((x `SC.fmul` x) `SC.fsub` x2) <> SC.zero then None
-           else (
-             let x = if (x % 2 = 1) <> sign then (SC.prime - x) % SC.prime else x in
-             Some x)
-             ))
-    )
-    (ensures  fun h0 _ h1 -> modifies (loc x |+| loc tmp) h0 h1 /\
-      F51.mul_inv_t h1 x /\
-      F51.fevalh h1 x == Some?.v (SE.recover_x (F51.as_nat h0 y) (uint_v #U64 sign <> 0))
-    )
+  (requires fun h ->
+    live h x /\ live h tmp /\ live h y /\
+    disjoint x y /\ disjoint tmp x /\ disjoint tmp y /\
+    F51.mul_inv_t h (gsub tmp 5ul 5ul) /\
+    (let y = F51.as_nat h y in
+    let sign = (uint_v #U64 sign <> 0) in
+    let x = F51.fevalh h (gsub tmp 5ul 5ul) in
+    let x2 = F51.fevalh h (gsub tmp  0ul 5ul) in
+    ((x `SC.fmul` x) `SC.fsub` x2) == SC.zero /\
+    SE.recover_x y sign ==
+      (if ((x `SC.fmul` x) `SC.fsub` x2) <> SC.zero then None
+      else (
+        let x =
+          if (x % 2 = 1) <> sign then (SC.prime - x) % SC.prime else x in
+        Some x))))
+  (ensures  fun h0 _ h1 -> modifies (loc x |+| loc tmp) h0 h1 /\
+    F51.mul_inv_t h1 x /\
+    F51.fevalh h1 x == Some?.v (SE.recover_x (F51.as_nat h0 y) (uint_v #U64 sign <> 0)))
 
 let recover_x_step_5 x y sign tmp =
   let x3  = sub tmp 5ul 5ul in
   let t0  = sub tmp 10ul 5ul in
-  let hi = ST.get() in
   reduce x3;
   let x0 = x_mod_2 x3 in
-  let h0 = ST.get() in
+
   let open Lib.RawIntTypes in
   let open FStar.UInt64 in
-  if not(u64_to_UInt64 x0 =^ u64_to_UInt64 sign) then (
+  if not (u64_to_UInt64 x0 =^ u64_to_UInt64 sign) then (
+    let h0 = ST.get () in
     make_zero t0;
-    fdifference x3 t0;
+    fdifference x3 t0 x3; // x3 = (-x) % prime
     reduce_513 x3;
     reduce x3;
     (**) assert_norm (SC.prime % SC.prime = SC.zero % SC.prime);
-    (**) FStar.Math.Lemmas.mod_add_both SC.prime SC.zero (- (F51.fevalh h0 x3)) SC.prime
-    );
+    (**) FStar.Math.Lemmas.mod_add_both SC.prime SC.zero (- (F51.fevalh h0 x3)) SC.prime);
   copy x x3
+
 
 inline_for_extraction noextract
 val recover_x_:
     x:elemB
   -> y:elemB
   -> sign:uint64{v sign = 0 \/ v sign = 1}
-  -> tmp:lbuffer uint64 20ul ->
+  -> tmp:lbuffer uint64 15ul ->
   Stack bool
     (requires fun h ->
       live h tmp /\ live h x /\ live h y /\
@@ -304,8 +270,6 @@ val recover_x_:
       (Some? res <==> z) /\
       (Some? res ==> F51.fevalh h1 x == Some?.v res))
     )
-
-#restart-solver
 
 let recover_x_ x y sign tmp =
   let x2 = sub tmp 0ul 5ul in
@@ -354,7 +318,7 @@ val recover_x:
 [@CInline]
 let recover_x x y sign =
   push_frame();
-  let tmp = create 20ul (u64 0) in
+  let tmp = create 15ul (u64 0) in
   let res = recover_x_ x y sign tmp in
   pop_frame();
   res
